Foundation/Propositional/Kripke/Hilbert/KC.lean
@@ -1,15 +1,18 @@
 import Foundation.Propositional.Hilbert.WellKnown
 import Foundation.Propositional.Kripke.AxiomWeakLEM
 import Foundation.Propositional.Kripke.Hilbert.Soundness
+import Foundation.Propositional.Kripke.Filteration
 
 namespace LO.Propositional
 
 open Kripke
 open Formula.Kripke
 
-namespace Hilbert.KC.Kripke
-
 instance : FrameClass.confluent.DefinedBy (Hilbert.KC.axioms) := FrameClass.definedBy_with_axiomEFQ inferInstance
+
+protected abbrev Kripke.FiniteFrameClass.confluent : FiniteFrameClass := { F | Confluent F.Rel }
+
+namespace Hilbert.KC.Kripke
 
 instance sound : Sound Hilbert.KC FrameClass.confluent := inferInstance
 
@@ -18,6 +21,29 @@ instance consistent : Entailment.Consistent Hilbert.KC := Kripke.Hilbert.consist
 instance canonical : Canonical Hilbert.KC FrameClass.confluent := ⟨Canonical.confluent⟩
 
 instance complete : Complete Hilbert.KC FrameClass.confluent := inferInstance
+
+section FFP
+
+instance sound_finite : Sound Hilbert.KC Kripke.FiniteFrameClass.confluent := ⟨by
+  intro φ hφ F hF;
+  apply Hilbert.finite_sound_of_sound sound |>.sound hφ;
+  simpa;
+⟩
+
+instance complete_finite : Complete (Hilbert.KC) Kripke.FiniteFrameClass.confluent := ⟨by
+  intro φ hφ;
+  apply Kripke.complete.complete;
+  rintro F hF V x;
+  let M : Kripke.Model := ⟨F, V⟩;
+  let FM := finestFilterationTransitiveClosureModel M ↑φ.subformulas;
+  apply filteration FM (finestFilterationTransitiveClosureModel.filterOf) (by simp) |>.mpr;
+  apply validOnModel_of_validOnFiniteFrameClass hφ;
+  . sorry;
+  . apply FilterEqvQuotient.finite;
+    simp;
+⟩
+
+end FFP
 
 end Hilbert.KC.Kripke
 
