Foundation/Propositional/Kripke/Hilbert/LC.lean
@@ -1,11 +1,16 @@
 import Foundation.Propositional.Hilbert.WellKnown
 import Foundation.Propositional.Kripke.AxiomDummett
 import Foundation.Propositional.Kripke.Hilbert.Soundness
+import Foundation.Propositional.Kripke.Filteration
 
 namespace LO.Propositional
 
 open Kripke
 open Formula.Kripke
+
+instance : FrameClass.connected.DefinedBy (Hilbert.LC.axioms) := FrameClass.definedBy_with_axiomEFQ inferInstance
+
+protected abbrev Kripke.FiniteFrameClass.connected : FiniteFrameClass := { F | Connected F.Rel }
 
 namespace Hilbert.LC.Kripke
 
@@ -18,6 +23,29 @@ instance consistent : Entailment.Consistent Hilbert.LC := Kripke.Hilbert.consist
 instance canonical : Canonical Hilbert.LC FrameClass.connected := ⟨Canonical.connected⟩
 
 instance complete : Complete Hilbert.LC FrameClass.connected := inferInstance
+
+section FFP
+
+instance sound_finite : Sound Hilbert.LC Kripke.FiniteFrameClass.connected := ⟨by
+  intro φ hφ F hF;
+  apply Hilbert.finite_sound_of_sound sound |>.sound hφ;
+  simpa;
+⟩
+
+instance complete_finite : Complete (Hilbert.LC) Kripke.FiniteFrameClass.connected := ⟨by
+  intro φ hφ;
+  apply Kripke.complete.complete;
+  intro F _ V x;
+  let M : Kripke.Model := ⟨F, V⟩;
+  let FM := finestFilterationTransitiveClosureModel M ↑φ.subformulas;
+  apply filteration FM (finestFilterationTransitiveClosureModel.filterOf) (by simp) |>.mpr;
+  apply validOnModel_of_validOnFiniteFrameClass hφ;
+  . sorry;
+  . apply FilterEqvQuotient.finite;
+    simp;
+⟩
+
+end FFP
 
 end Hilbert.LC.Kripke
 
